\documentclass{article}

\usepackage{amsfonts}
\usepackage{amsmath}
\usepackage{amssymb}
\usepackage{graphicx}
\usepackage{graphicx}
\usepackage{xcolor}

\begin{document}

\newcommand{\R}{\mathbb{R}}

\title{HW4 MATH 670}
\author{Fernando}
\date{\today}
\maketitle

\section*{\#1}
Let's do it by induction on \(k\). For \(k=1\)
\[
  Fl(d_1)\simeq Gr(d_1,\mathbb{R}^n)
\]
and on example 3.12.9 of the notes we have the result.
Now we assume the result for \(k\) and prove it for \(k+1\), i.e.
\[
  Fl(d_1,\dots,d_{k+1})\simeq O(n)/(O(n_1)\times\dots\times O(n_{k+1}))
\]
We can decompose a flag as
\[
  \{<u_1,\dots,u_{d_1}>,\dots,<u_1,\dots,u_{d_{k+1}}>\}
\]
the last space is
\[
  <u_1,\dots,u_{d_k}>\oplus<u_{d_k+1},\dots,u_{d_k+1}>
\]
We only need a new \(O(n_{k+1})\) to fix the new term in the direct sum. Therefore taking the quotient by this new factor gives the result
by the third isomorphism theorem.
\section*{\#2}
We can write the vector field in local coordinates like this
\[
  V=\sum v_kX_k
\]
then
\[
  V'(t)=\sum v_k'(t)X_k.
\]
On the other hand
\[
  \frac{DV}{dt}=\sum_{i,j,k}\left(\frac{dv_k}{dt}+\frac{d\alpha_i}{dt}v_j\Gamma^k_{ij}\right)X_k.
\]
In this case \(\frac{\partial d\alpha_i}{dt}=0\), so it doesn't matter what \(\Gamma^k_{ij}\) is. We will get:
\[
  \frac{DV}{dt}=\sum\frac{dv_k}{dt}X_k=\sum v_k'(t)X_k=V'(t).
\]
\section*{\#3}

\(\implies\)

Let's take an orthonormal basis for \(T_{\alpha(t_0)}M\):
\[\{v_1(t_0),\dots,v_n(t_0)\}\]
Since \(\nabla\) is compatible with \(g\) we can parallel transport this basis along \(\alpha\),
then
\[
  span\{v_1(t),\dots,v_n(t)\}=T_{\alpha(t)}M,
\]
so we can write \( V(t)=\sum\beta_iv_i(t), W(t)=\sum\gamma_iv_i(t)
\) for \(\beta_i,\gamma_i\) smooth functions.

now we see that
\begin{align}
  \label{eq:LHS}
  \frac{d}{dt}\bigg|_{t=t_0}g_{\alpha(t)}(V(t),W(t))&=\sum_{ij}
  \frac{d}{dt}\bigg|_{t=t_0}\beta_i\gamma_ig_{\alpha(t)}(v_i(t),v_j(t)) \nonumber\\
  &=\sum\frac{d}{dt}\bigg|_{t=t_0}\beta_i\gamma_i \nonumber\\
  &=\sum\gamma_i\frac{d\beta_i}{dt}\bigg|_{t=t_0}+\sum\beta_i\frac{d\gamma_i}{dt}\bigg|_{t=t_0}
\end{align}

On the other hand we have
\begin{align}
  \label{eq:RHS}
  &g_{\alpha(t_0)}\left(\frac{dV}{dt},W(t)\right) + g_{\alpha(t_0)}\left(V(t),\frac{DW}{dt}\right) \nonumber\\
  &= g_{\alpha(t_0)}\left(\sum\beta_i'v_i(t),W(t)\right) + g_{\alpha(t_0)}\left(V(t),\sum\gamma_i'v_i(t)\right)\nonumber\\
  &= \sum g_{\alpha(t_0)}\left(\beta_i'v_i(t),W(t)\right) + \sum g_{\alpha(t_0)}\left(V(t),\gamma_i'v_i(t)\right)\nonumber\\
  &= \sum\gamma_i\frac{d\beta_i}{dt}\bigg|_{t=t_0} + \sum\beta_i\frac{d\gamma_i}{dt}\bigg|_{t=t_0}
\end{align}
So by \eqref{eq:LHS} and \eqref{eq:RHS} we have the result.

\(\impliedby\)

Let \(V,W\) be parallel along \(\alpha\), then \(\frac{DV}{dt}=0=\frac{DW}{dt}\), so
\begin{align*}
  \frac{d}{dt}\bigg|_{t=t_0}g_{\alpha(t)}(V(t),W(t))&=g_{\alpha(t)}\left(\frac{DV}{dt},W\right)+g_{\alpha(t)}\left(V,\frac{DW}{dt}\right)\\
  &=g_{\alpha(t)}\left(0,W\right)+g_{\alpha(t)}\left(V,0\right)\\
  &=0.
\end{align*}
i.e. \(g_{\alpha(t)}(V(t),W(t))\) is constant.

\end{document}
